theories/coneris/lib/hocap_rand'.v
@@ -1,0 +1,243 @@
+(** * Hocap rand that generates a exclusive token as well
+      Useful for building more complex data structures when we need to know all the tapes generated
+      We also fix the tape bound
+ *)
+From iris.algebra Require Import excl_auth gmap.
+From clutch.coneris Require Import coneris abstract_tape.
+
+Set Default Proof Using "Type*".
+
+Class rand_spec' (tb:nat) `{!conerisGS Σ} := RandSpec'
+{
+  (** * Operations *)
+  rand_allocate_tape : val;
+  rand_tape : val;
+  (** * Ghost state *)
+
+  rand_tape_name: Type;
+  
+  (** * Predicates *)
+  is_rand (N:namespace)
+    (γ1: rand_tape_name) : iProp Σ; 
+  (* rand_tapes_auth {L : randG Σ} (γ: rand_tape_name) (m:gmap loc (nat * list nat)): iProp Σ; *)
+  rand_tapes (* (γ: rand_tape_name) *) (α:val) (ns: (list nat)) (γ1: rand_tape_name): iProp Σ;
+  rand_token (α: val) (γ:rand_tape_name) : iProp Σ;
+  (** * General properties of the predicates *)
+  #[global] is_rand_persistent N γ1 ::
+    Persistent (is_rand N γ1);
+  (* #[global] rand_tapes_auth_timeless {L : randG Σ} γ m :: *)
+  (*   Timeless (rand_tapes_auth (L:=L) γ m); *)
+  #[global] rand_tapes_timeless α ns γ::
+    Timeless (rand_tapes α ns γ);  
+  #[global] rand_token_timeless α γ::
+    Timeless (rand_token α γ);  
+  (* #[global] rand_tape_name_inhabited :: *)
+  (*   Inhabited rand_tape_name; *)
+
+  (* rand_tapes_auth_exclusive {L : randG Σ} γ m m': *)
+  (* rand_tapes_auth (L:=L) γ m -∗ rand_tapes_auth (L:=L) γ m' -∗ False; *)
+  rand_tapes_exclusive α ns ns' γ:
+  rand_tapes α ns γ-∗ rand_tapes α ns' γ-∗ False;
+  rand_token_exclusive α γ:
+  rand_token α γ -∗ rand_token α γ -∗ False; 
+  (* rand_tapes_agree {L : randG Σ} γ α m ns: *)
+  (* rand_tapes_auth (L:=L) γ m -∗ rand_tapes (L:=L) γ α ns -∗ ⌜ m!! α = Some (ns) ⌝; *)
+  rand_tapes_valid α ns γ:
+    rand_tapes α ns γ -∗ ⌜Forall (λ n, n<=tb)%nat ns⌝ ; 
+  (* rand_tapes_update {L : randG Σ} γ α m ns ns': *)
+  (* Forall (λ x, x<=ns'.1) ns'.2 -> *)
+  (*   rand_tapes_auth (L:=L) γ m -∗ rand_tapes (L:=L) γ α ns ==∗ *)
+  (*   rand_tapes_auth (L:=L) γ (<[α := ns']> m) ∗ rand_tapes (L:=L) γ α ns'; *)
+  rand_tapes_presample N E α ns ε (ε2 : fin (S tb) -> R) γ:
+  ↑N⊆E -> 
+  (∀ x, 0<=ε2 x)%R ->
+  (SeriesC (λ n, 1 / (S tb) * ε2 n)%R <= ε)%R ->
+  is_rand N γ -∗
+  rand_tapes α ns γ-∗
+  ↯ ε  -∗
+  state_update E E (∃ n, ↯ (ε2 n) ∗ rand_tapes α (ns ++ [fin_to_nat n]) γ); 
+    
+
+  (** * Program specs *)
+  rand_inv_create_spec N E:
+  ↑N ⊆ E -> ⊢ |={E}=> (∃ γ1, is_rand N γ1);
+  
+  rand_allocate_tape_spec N γ E :
+  ↑N ⊆ E ->
+    {{{ is_rand N γ }}}
+      rand_allocate_tape #() @ E
+      {{{ (v:val), RET v;
+          rand_token v γ∗
+           rand_tapes v [] γ
+      }}}; 
+  
+  rand_tape_spec_some N γ E α n ns:
+  ↑N ⊆ E ->
+    {{{ is_rand N γ ∗ rand_tapes α (n::ns) γ }}}
+      rand_tape α @ E
+                       {{{ RET #n; rand_tapes α (ns) γ }}}; 
+}.
+
+Section impl1.
+  Context `{!conerisGS Σ, Hs : !ghost_mapG Σ val (), Hm : !abstract_tapesGS Σ }.
+  Variable tb:nat.
+  Local Opaque INR.
+  (* (** Instantiate rand *) *)
+  Local Definition rand_inv_pred1  (γ:gname*gname) : iProp Σ:=
+    (∃ (m:gmap val (list nat)),
+        (ghost_map_auth γ.1 1 ((λ _, ())<$>m)) ∗
+        ● ((λ x, (tb, x))<$>m)@ γ.2 ∗
+        [∗ map] α ↦ns∈m, (∃ α', ⌜α = #lbl:α'⌝ ∗ (α' ↪N (tb; ns) ))
+    )%I.
+
+  Definition is_rand1 N γ:=
+    inv N (rand_inv_pred1 γ).
+
+  Definition rand_tapes1 α ns (γ:gname*gname):=
+    (α◯↪N (tb; ns) @γ.2 ∗ ⌜Forall (λ x, x<=tb)%nat ns⌝)%I.
+
+  Definition rand_token1 α (γ:gname*gname) :=
+    (α ↪[γ.1] ())%I.
+  
+  #[local] Program Definition rand_spec1 : rand_spec' tb :=
+    {| rand_allocate_tape:= (λ: "_", alloc #tb);
+      rand_tape:= (λ: "α", rand("α") #tb); 
+      is_rand  := is_rand1;
+      rand_tapes := rand_tapes1;
+      rand_token := rand_token1;
+    |}.
+  Next Obligation.
+    simpl.
+    iIntros (????) "[H1 %] [H2 %]".
+    iApply (abstract_tapes_frag_exclusive with "[$][$]").
+  Qed.
+  Next Obligation.
+    simpl.
+    iIntros (??) "H1 H2".
+    iCombine "H1 H2" gives "%H".
+    cbv in H. naive_solver.
+  Qed.
+  Next Obligation.
+    simpl.
+    iIntros (???) "(?&$)". 
+  Qed.
+  Next Obligation.
+    simpl.
+    iIntros (??????????) "#Hinv [H1 %] Herr".
+    iInv "Hinv" as ">(%&Hs&Hm&Ht)" "Hclose".
+    iDestruct (abstract_tapes_agree with "[$][$]") as "%Hsome".
+    rewrite lookup_fmap_Some in Hsome.
+    destruct Hsome as (?&?&Hsome). simplify_eq.
+    iDestruct (big_sepM_insert_acc with "[$]") as "[(%&%Heq&Ht) Hclose']"; first done.
+    simplify_eq.
+    iMod (state_update_presample_exp with "[$][$]") as "(%n&Ht&Herr)"; [done..|].
+    iMod (abstract_tapes_presample with "[$][$]") as "[Hm H1]".
+    iDestruct ("Hclose'" with "[$Ht]") as "Ht"; first done.
+    iMod ("Hclose" with "[Hs Hm $Ht]"); last iFrame.
+    - rewrite !fmap_insert (insert_id _ _ ()); first iFrame.
+      rewrite lookup_fmap. by rewrite Hsome.
+    - iPureIntro. apply Forall_app; split; first done.
+      apply Forall_singleton. pose proof fin_to_nat_lt n. lia.
+  Qed.
+  Next Obligation.
+    iIntros (???).
+    rewrite /is_rand1/rand_inv_pred1.
+    iMod (abstract_tapes_alloc ∅) as "(%&H1&_)".
+    iMod (ghost_map_alloc_empty) as "(%&H2)".
+    iMod (inv_alloc with "[H1 H2]"); last first.
+    - iExists (_,_). by iFrame.
+    - iNext. iExists ∅.
+      rewrite !fmap_empty. by iFrame.
+  Qed.
+  Next Obligation.
+    simpl.
+    iIntros (?[??]?? Φ) "#Hinv HΦ".
+    wp_pures.
+    iInv "Hinv" as ">(%&Hs&Hm&Hts)" "Hclose".
+    wp_apply (wp_alloc_tape); first done.
+    iIntros (α) "Ht".
+    iAssert (⌜m!!#lbl:α=None⌝)%I as "%Hnone".
+    { destruct (_!!_) eqn:?; last done.
+      iDestruct (big_sepM_insert_acc with "[$]") as "[(%&%&?) Hclose']"; first done.
+      simplify_eq.
+      by iDestruct (tapeN_tapeN_contradict with "[$][$]") as "%".
+    }
+    iMod (ghost_map_insert with "[$]") as "[Hs Htoken]"; first by erewrite lookup_fmap, Hnone.
+    iMod (abstract_tapes_new with "[$]") as "[Hm ?]"; first by erewrite lookup_fmap, Hnone.
+    iMod ("Hclose" with "[Hts Ht Hs Hm]").
+    { iNext. iExists (<[_:=_]>_). rewrite !fmap_insert.
+      iFrame.
+      rewrite big_sepM_insert; last done.
+      by iFrame.
+    }
+    iApply "HΦ". by iFrame.
+  Qed.
+  Next Obligation.
+    iIntros (?[??]???? Hsubset Φ) "[#Hinv [Htfrag %]] HΦ".
+    iApply fupd_pgl_wp.
+    iInv "Hinv" as ">(%&Hs&Hm&Hts)" "Hclose".
+    iDestruct (abstract_tapes_agree with "[$][$]") as "%Hsome".
+    rewrite lookup_fmap_Some in Hsome.
+    destruct Hsome as (?&?&?). simplify_eq.
+    iDestruct (big_sepM_lookup_acc with "[$]") as "[(%&%&?) Hclose']"; first done.
+    simplify_eq.
+    iMod ("Hclose" with "[-Htfrag HΦ]") as "_"; iFrame.
+    { iDestruct ("Hclose'" with "[-]") as "$". by iFrame. }
+    iModIntro. wp_pures.
+    iInv "Hinv" as ">(%&Hs&Hm&Hts)" "Hclose".
+    iDestruct (abstract_tapes_agree with "[$][$]") as "%Hsome".
+    rewrite lookup_fmap_Some in Hsome.
+    destruct Hsome as (?&?&Hsome). simplify_eq.
+    iDestruct (big_sepM_insert_acc with "[$]") as "[(%&%&?) Hclose']"; first done.
+    simplify_eq.
+    wp_apply (wp_rand_tape with "[$]") as "[Htape %]".
+    iMod (abstract_tapes_pop with "[$][$]") as "[Hm Htfrag]".
+    iDestruct ("Hclose'" with "[$Htape]") as "Htapes"; first done.
+    iMod ("Hclose" with "[-HΦ Htfrag]").
+    { iFrame. rewrite !fmap_insert. iFrame.
+      rewrite (insert_id _ _ ()); first iFrame.
+      rewrite lookup_fmap. by rewrite Hsome. }
+    iApply "HΦ". iFrame.
+    iPureIntro. by eapply Forall_inv_tail.
+  Qed.
+End impl1.
+
+Section checks.
+  Context `{H: conerisGS Σ, r1:!rand_spec' tb}.
+  
+  Lemma wp_rand_tape_1 N n ns α γ:
+    {{{ is_rand N γ ∗ ▷ rand_tapes α (n :: ns) γ }}}
+      rand_tape α 
+                       {{{ RET #(LitInt n); rand_tapes α (ns) γ ∗ ⌜n <= tb⌝ }}}.
+  Proof.
+    iIntros (Φ) "[#Hinv >Hfrag] HΦ".
+    iDestruct (rand_tapes_valid with "[$]") as "%H'". 
+    wp_apply (rand_tape_spec_some with "[$Hfrag //]"); first exact.
+    iIntros.
+    iApply "HΦ".
+    iFrame.
+    iPureIntro.
+    rewrite Forall_cons in H'. naive_solver.
+  Qed.
+
+  Local Opaque enum_uniform_fin_list.
+
+              
+  Lemma wp_presample_adv_comp_rand_tape N E α ns (ε1 : R) (ε2 : fin (S tb) -> R) γ:
+    ↑N ⊆ E ->
+    (∀ n, 0<=ε2 n)%R ->
+    (SeriesC (λ n, (1 / (S tb)) * ε2 n)%R <= ε1)%R →
+    is_rand N γ -∗
+    ▷ rand_tapes α (ns) γ -∗
+    ↯ ε1 -∗
+    wp_update E (∃ n, ↯ (ε2 n) ∗ rand_tapes α (ns ++[fin_to_nat n]) γ)%I.
+  Proof.
+    iIntros (Hsubset Hpos Hineq) "#Hinv >Htape Herr".
+    iDestruct (ec_valid with "[$]") as "%Hpos'".
+    destruct Hpos' as [Hpos' ?].
+    iApply wp_update_state_update.
+    by iApply (rand_tapes_presample with "[$][$]").
+  Qed.
+      
+
+End checks.
